last commit before transition to fold_right in SAT.v

theories/L/Complexity/MorePrelim.v
@@ -1,5 +1,7 @@
 Require Import PslBase.Base.
 Require Import Lia. 
+From Undecidability.L Require Import L.
+From Undecidability.Shared Require Import Prelim.
 
 Section pair_eq.
   Variable (X Y : Type). 
@@ -17,6 +19,88 @@ Section pair_eq.
       apply eqbX_correct; congruence. apply eqbY_correct; congruence. 
     + intros [H1 H2]%andb_prop. apply eqbX_correct in H1. apply eqbY_correct in H2. congruence. Qed. 
 End pair_eq. 
+
+(** *Results regarding lists *)
+
+Section takeN.
+  Variable (X : Type).
+  Fixpoint takeN (l : list X) (n : nat) {struct n} :=
+    match n with 0 => []
+               | S n => match l with [] => []
+                           | (l :: ls) => l :: takeN ls n
+                        end
+    end. 
+
+  Lemma ntherror_sublist (l l' : list X) (k : nat) (x : X) : (nth_error l k = Some x) -> nth_error (l ++ l') k = Some x. 
+  Proof. 
+    revert k. 
+    induction l. 
+    - intros []; cbn; congruence.  
+    - intros k H. destruct k.
+      + cbn in H. destruct l'; now cbn.
+      + cbn. apply IHl. now cbn in H. 
+  Qed. 
+
+  Lemma takeN_sublist (l : list X) (k k' : nat) (t : list X) : takeN l k = t -> k' >= k -> exists t', takeN l k' = t ++ t'. 
+  Proof. 
+    revert k k' t. induction l. 
+    - intros k k' t H1 H2. exists []. destruct k', k; cbn in H1; cbn; rewrite <- H1; firstorder. 
+    - intros k k' t H1 H2. destruct k, k'; cbn in H1; cbn; try rewrite <- H1. firstorder.
+      exists (a :: takeN l k'). firstorder. lia.
+      destruct t; try congruence. 
+      specialize (IHl k k' t). inv H1.  destruct (IHl); try tauto; try lia. exists x0. cbn. now rewrite <- H. 
+  Qed. 
+
+  Lemma takeN_more_length (l : list X) (k : nat) : k >= (|l|) ->  takeN l k = l. 
+  Proof. 
+    revert k. induction l. 
+    - intros k. cbn. destruct k; tauto. 
+    - intros k. cbn. destruct k; cbn. lia. intros H. rewrite IHl. reflexivity. lia. 
+  Qed. 
+
+  Lemma takeN_split (l : list X) (k : nat) : exists t, l = takeN l k ++ t.
+  Proof.
+    enough (exists t, takeN l (|l|) = takeN l k ++ t). 
+    { destruct H. specialize (@takeN_more_length l (|l|)) as H2. exists x. rewrite <- H, H2; [reflexivity | lia]. }
+    destruct (lt_eq_lt_dec k (|l|)) as [[H|H] |H].
+    1-2: apply takeN_sublist with (k:=k); try reflexivity; try lia.  
+    exists []. repeat rewrite takeN_more_length. firstorder. all: lia.
+  Qed. 
+
+  Lemma takeN_length (l :list X) (k : nat) : (|takeN l k|) <= k. 
+  Proof. 
+    induction l in k |-*. 
+    - destruct k; cbn; lia. 
+    - destruct k; cbn; try lia. rewrite IHl. lia. 
+  Qed. 
+
+  Lemma takeN_minlength (l : list X) (n k : nat) : |l| >= k -> n >= k -> |takeN l n| >= k. 
+  Proof. 
+    induction l in n, k |-*. 
+    - destruct n; cbn; lia.
+    - cbn. destruct n, k; cbn. 1-3: lia.
+      intros H1 H2. enough (|takeN l n| >= k) by lia. apply IHl; lia.  
+  Qed. 
+
+  Lemma ntherror_take (l : list X) (k n : nat) (v :X) : k < n -> nth_error l k = Some v -> nth_error (takeN l n) k = Some v. 
+  Proof. 
+    specialize (takeN_split l n) as [t H]. intros H1 H2. 
+    (*Proof by contradiction*)
+    destruct (nth_error (takeN l n) k) eqn:H3. 
+    2: { exfalso. 
+        apply nth_error_None in H3. assert (|l| > k) by (now apply nth_error_Some_lt with (x := v)).
+        (*contradiction by H1, H3, H0 *)
+        destruct (takeN_split l k) as [[] H4].
+        - enough (|l| = k) by lia. rewrite H4. enough (|takeN l k| <= k /\ |takeN l k| >= k).
+          {replace (takeN l k ++ []) with (takeN l k) by firstorder. lia. }
+          split. apply takeN_length. apply takeN_minlength. all: lia. 
+        - assert (|takeN l n| = k). enough (|takeN l n| >= k) by lia. apply takeN_minlength; lia. 
+          assert (|takeN l n| >= S k). apply takeN_minlength; lia. lia. 
+    }
+    rewrite H in H2. specialize(Prelim.nthe_app_l t H3) as H4. now rewrite H4 in H2. 
+  Qed. 
+End takeN.
+
 
 Section subsequence.
   Variable (X : Type).
