theories/L/Complexity/PolyBounds.v
@@ -143,6 +143,85 @@ Section fixX.
   Qed. 
 End fixX.
 
+Section fixXY.
+  Context {X Y Z: Type}.
+  Context {H:registered X}.
+  Context {H0: registered Y}.
+  Context {H1 : registered Z}.
+
+    Fixpoint fold_right_time (f : Y -> X -> X) (tf : timeComplexity (Y -> X -> X)) (l : list Y) (acc : X) :=
+      match l with [] => 4
+              | l::ls => callTime2 tf l (fold_right f acc ls) + 15 + fold_right_time f tf ls acc
+      end. 
+  Instance term_fold_right : computableTime' (@fold_right X Y) (fun f fT => (1, fun acc _ => (1, fun l _ => (fold_right_time f fT l acc + 4, tt)))).
+  Proof.
+    extract. solverec. unfold fold_right. solverec.  
+  Qed. 
+
+  Lemma fold_right_time_bound_env (step : Z -> Y -> X -> X) (stepT : Z -> timeComplexity (Y -> X -> X)) :
+    (exists (f : nat -> nat), (forall (acc : X) (ele : Y) (env : Z), callTime2 (stepT env) ele acc <= f(size(enc acc) + size(enc ele) + size(enc env))) /\ inOPoly f /\ monotonic f)
+    -> (exists (c__out : nat), forall (acc : X) (ele : Y) (env : Z), size(enc (step env ele acc)) <= size(enc acc) + size(enc ele) + size(enc env) + c__out)
+    -> exists (f : nat -> nat), (forall (l : list Y) (acc : X) (env : Z), fold_right_time (step env) (stepT env) l acc <= f(size(enc l) + size(enc acc) + size(enc env))) /\ inOPoly f /\ monotonic f.
+  Proof.
+    intros (f__step & H2 & H3 & H4) (c__out & F). 
+    evar (f : nat -> nat). exists f. split.
+    - intros l init env.
+      (* we first show that the output size of foldr on every suffix is polynomial *)
+      assert (forall l' l'', l = l' ++ l'' -> size(enc (fold_right (step env) init l'')) <= size(enc init) + size(enc l'') + (|l''|) * (size(enc env) + c__out)).
+      {
+        intros l' l''; revert l'. induction l''.
+        + cbn. intros; lia.
+        + intros. cbn. rewrite F. rewrite IHl''. 2: { now rewrite app_comm_cons' in H5. }
+          rewrite list_size_cons. solverec. 
+      }
+
+      instantiate (f := fun n => 4 + n * f__step((S c__out) * n * n + n) + 15 * n). subst f.
+      unfold fold_right_time. 
+      induction l.
+      + solverec.
+      + rewrite IHl, H2.
+        * unfold monotonic in H4.
+          rewrite H4 with (x' := size(enc init) + size(enc l) + (|l|) * (size(enc env) + c__out) + size(enc a) + size(enc env)). 2: rewrite H5; [lia|assert (a::l = [a] ++ l) as H6 by reflexivity; apply H6].
+
+          rewrite H4 with (x' := (S c__out) * (size(enc(a::l)) + size(enc init) + size(enc env)) *  (size(enc(a::l)) + size(enc init) + size(enc env)) + (size(enc(a::l)) + size(enc init) + size(enc env))). 
+          2: {clear IHl. rewrite list_size_length. rewrite list_size_cons. cbn; nia. }
+
+          setoid_rewrite H4 with (x' := (S c__out) *( size(enc(a::l)) + size(enc init) + size(enc env)) *  (size(enc(a::l)) + size(enc init) + size(enc env)) + (size(enc(a::l)) + size(enc init) + size(enc env))) at 2. 
+          2: {clear IHl. rewrite list_size_cons. cbn; nia. }
+
+          rewrite list_size_cons at 7. rewrite list_size_cons at 10. solverec. 
+       * clear IHl. intros. apply H5 with (l' := a::l'). firstorder. 
+  - subst f; split; smpl_inO. apply inOPoly_comp; smpl_inO. 
+Qed. 
+
+
+  (*the running time of foldl not only depends on the running time of the step function, *)
+  (*but also on the output size of the step function; in order to get a polynomial bound, *)
+  (*we require that this output size grows only by an additive constant in each step *)
+  Lemma fold_left_time_bound_env (step : Z -> X -> Y -> X) (stepT : Z -> timeComplexity (X -> Y -> X)) :
+    (exists (f : nat -> nat), (forall (acc : X) (ele : Y) (env : Z), callTime2 (stepT env) acc ele <= f(size(enc(acc)) + size(enc ele) + size(enc env))) /\ inOPoly f /\ monotonic f)
+    -> (exists (c__out : nat), forall (acc : X) (ele : Y) (env : Z), size(enc (step env acc ele)) <= size(enc acc) + size(enc ele) + size(enc env) + c__out)
+    -> exists (f : nat -> nat), (forall (l : list Y) (acc : X) (env : Z), fold_left_time (step env) (stepT env) l acc <= f(size(enc l) + size(enc acc) + size(enc env))) /\ inOPoly f /\ monotonic f. 
+  Proof.
+    intros (f__step & H2 & H3 & H4) (c__out & F). 
+    evar (f : nat -> nat). exists f. split.
+    - intros l init env.  
+      (*we strengthen the statement: for every acc that is polynomial in init, l and env, we derive the bound*)
+      (* enough (forall acc, (exists f__acc, size(enc acc) <= f__acc(size(enc init) + size(enc l) + size(enc env)) /\ inOPoly f__acc /\ monotonic f__acc) -> fold_left_time (step env) (stepT env) l acc <= f (size(enc l) + size(enc init) + size(enc env))). *)
+      (* {apply (H5 init). exists (fun n => n); split; [lia |split; smpl_inO]. } *)
+      revert init.
+      instantiate (f := fun n => 4 + 15 * n + n * f__step(n * n + (1 + c__out) * n)). subst f. 
+      induction l. 
+      + intros. solverec. 
+      + intros acc. unfold fold_left_time. fold (@fold_left_time X Y). 
+        rewrite IHl. rewrite H2. rewrite F.
+        (*we'd like to rewrite with G1, but can't do that directly since we have no Proper instance for monotonic functions *)
+        unfold monotonic in H4. rewrite H4 with (x' := f__acc (size(enc init) + size(enc (a::l)) + size(enc env)) + size(enc a) + size(enc env)). 2: now rewrite G1.
+        
+
+
+
+
 (*We now fix variants where the environment is not important*)
 Require Import Undecidability.L.Datatypes.LUnit.
 Section noEnv.
