theories/L/Complexity/Problems/SAT.v
@@ -1,7 +1,7 @@
 From Undecidability.L Require Import L.
 From Undecidability.L.Tactics Require Import LTactics ComputableTactics.
 From Undecidability.L.Datatypes Require Import LProd LTerm LNat Lists LOptions.
-From Undecidability.L.Complexity Require Import NP Synthetic Monotonic Tactics PolyBounds.
+From Undecidability.L.Complexity Require Import NP Synthetic Monotonic Tactics PolyBounds MorePrelim.
 From Undecidability.L.Functions Require Import Size.
 
 (*Conjunctive normal forms (need not be canonical)*)
@@ -30,6 +30,15 @@ Proof.
     + now apply H. 
     + apply IHc. firstorder.
 Qed. 
+
+Lemma varBound_clause_monotonic (c : clause) (n n' : nat) : n <= n' -> varBound_clause n c -> varBound_clause n' c. 
+Proof. intros H1 H2. induction H2. constructor. constructor. lia. auto. Qed. 
+
+Lemma varBound_cnf_monotonic (c : cnf) (n n' : nat) : n <= n' -> varBound_cnf n c -> varBound_cnf n' c.
+Proof.
+  intros H1 H2. induction H2; constructor.
+  now apply varBound_clause_monotonic with (n:= n). assumption. 
+Qed.
 
 (*Assignments as lists of natural numbers: variable i is mapped to value list[i] *)
 Notation assgn := (list bool). 
@@ -83,13 +92,11 @@ Qed.
 
 Lemma evalClause'_correct (l : clause) (a : assgn) (n : nat) (b : bool): varBound_clause n l -> |a| >= n -> exists v, evalClause' a l (Some b) = Some v. 
 Proof. 
-  intros H1; revert b; induction l. 
-  - intros b _. cbn; eauto. 
-  - intros b' H2. inv H1. unfold evalClause'.
-    destruct (evalLiteral_correct b H3 H2) as [v H0].
-    unfold fold_leftOption. rewrite H0.  fold fold_leftOption.  
-    destruct (IHl H4 (b' || v) H2) as [v' H1]. 
-    exists v'. auto. 
+  intros H1; revert b; induction H1. 
+  - intros; cbn. now exists b.
+  - intros. unfold evalClause', fold_leftOption. 
+    destruct (evalLiteral_correct b H H0) as [v H2]. rewrite H2.
+    destruct (IHvarBound_clause (b0||v) H0) as [v' H3]. exists v'; auto. 
 Qed. 
 
 Corollary evalClause_correct (l : clause) (a : assgn) (n : nat) : varBound_clause n l -> |a| >= n -> exists v, evalClause a l = Some v. 
@@ -99,13 +106,10 @@ Qed.
 
 Lemma evalCnf'_correct (l : cnf) (a : assgn) (n : nat) (b : bool): varBound_cnf n l -> |a| >= n -> exists v, evalCnf' a l (Some b) = Some v. 
 Proof. 
-  intros H1; revert b; induction l. 
-  - intros b _. cbn; eauto. 
-  - intros b H2. inv H1. unfold evalCnf'. 
-    destruct (evalClause_correct H3 H2) as [v H0]. 
-    unfold fold_leftOption. rewrite H0. fold fold_leftOption. 
-    destruct (IHl H4 (b && v) H2) as [v' H1]. 
-    exists v'. auto. 
+  intros H1; revert b. induction H1. 
+  - intros. cbn. now exists b.
+  - intros. cbn. destruct (evalClause_correct H H0) as [v H2]. 
+    rewrite H2. destruct (IHvarBound_cnf (b && v) H0) as [v' H3]. exists v'. auto.  
 Qed.
 
 (* inversion of evaluation*)
@@ -165,6 +169,47 @@ Lemma evalCnf_iff_bound (a :assgn) (c : cnf) : (exists v, evalCnf a c = Some v) 
 Proof. 
   split; eauto using evalCnf_varBound. 
   intros (n & H1 & H2). now apply evalCnf_correct with (n:= n). 
+Qed. 
+
+(*A computable notion of boundedness *)
+(*fold_left makes verification more ugly, but the runtime functions get easier *)
+Definition clause_maxVar (c : clause) := fold_left (fun acc '(_, v) => Nat.max acc v) c 0. 
+Definition cnf_maxVar (c : cnf) := fold_left (fun acc cl => Nat.max acc (clause_maxVar cl)) c 0.
+
+Lemma clause_maxVar_bound (c : clause) : varBound_clause (S (clause_maxVar c)) c. 
+Proof.
+  induction c.
+  - cbn. constructor. 
+  - destruct a. constructor. cbn.
+    1: { clear IHc. revert n; induction c. 
+         + intros; cbn; lia.
+         + intros; cbn. destruct a. specialize (IHc (Nat.max n n0)); lia. 
+       } 
+    eapply varBound_clause_monotonic.
+    2: apply IHc. unfold clause_maxVar. cbn. 
+    clear IHc. assert (n >= 0) by lia. revert n H. generalize 0.
+    induction c.
+    + intros; cbn. lia. 
+    + intros; cbn. destruct a. apply IHc. lia.  
+Qed. 
+
+Lemma cnf_maxVar_bound (c : cnf) : varBound_cnf (S (cnf_maxVar c)) c.
+Proof.
+  induction c.
+  - cbn; constructor. 
+  - constructor.
+    1: { cbn. eapply varBound_clause_monotonic. 2: apply clause_maxVar_bound.
+         clear IHc. generalize (clause_maxVar a). induction c.
+         + intros n; cbn; lia. 
+         + intros n; cbn. specialize (IHc (max n (clause_maxVar a0))). lia.  
+       } 
+    eapply varBound_cnf_monotonic. 2: apply IHc. cbn. unfold cnf_maxVar.  
+    pose (step := (fun acc (cl :list (bool * nat)) => Nat.max acc (clause_maxVar cl)) ). 
+    enough (forall n n', n >= n' -> fold_left step c n' <= fold_left step c n).  
+    {assert (0 <= (clause_maxVar a)) by lia. specialize (H (clause_maxVar a) 0 H0). subst step. lia. }
+    clear IHc. induction c. 
+    + intros n n' H. cbn; lia. 
+    + intros n n' H. cbn. apply IHc. unfold step; lia. 
 Qed. 
 
 
@@ -247,12 +292,12 @@ Proof.
     + intros H. split. 2: now apply evalClause_varBound.
       apply evalClause_step_inv in H. destruct H as (b1 & b2 & H1 & H2 & H3). destruct b2.
       * exists a0. firstorder. 
-      * destruct b1. 2: discriminate H3. apply IHcl in H1. destruct H1 as [[l [F1 F2]] _]. exists l. firstorder. 
+      * destruct b1. 2: discriminate H3. apply IHcl in H1. destruct H1 as [[l [F1 F2]] _]. exists l. split; [now right | assumption]. 
     + intros [(l & H1 & H2) H]. destruct H1.
       * rewrite H0 in *. cbn; rewrite H2. change (evalClause' a cl (Some true) = Some true).
         apply evalClause'_init_true. now inv H. 
       * cbn. destruct (evalLiteral a a0) eqn:eq. destruct b.
-        change (evalClause' a cl (Some true) = Some true). rewrite evalClause'_init_true. reflexivity. now inv H. 
+        change (evalClause' a cl (Some true) = Some true). rewrite evalClause'_init_true. reflexivity. now inv H.
         change (evalClause a cl = Some true). apply IHcl. split. exists l. firstorder. now inv H. 
         inv H. assert (|a| >= |a|) by lia. specialize (evalLiteral_correct b H4 H) as (v & H6). congruence. 
 Qed. 
@@ -271,6 +316,67 @@ Qed.
 
 Definition SAT (c : cnf) : Prop := exists (a : assgn), evalCnf a c = Some true. 
 
+(*a verifier for SAT. The condition |a| <= S(cnf_maxVar cn) is needed in order to make sure that it rejects certificates that are too long*)
+Definition sat_verifier (cn : cnf) (a : assgn) :=
+  evalCnf a cn = Some true /\ |a| <= S(cnf_maxVar cn).
+
+(*tools needed for the verification of the verifier*)
+(*now the wanted results: we can shorten the assignment if this doesn't yield to variables being unbound*)
+Lemma bounded_cap_assgn_literal (n : nat) (sgn : bool) (k : nat) : n < k ->
+  forall (a : assgn) (v : bool), evalLiteral a (sgn, n) = Some v -> evalLiteral (takeN a k) (sgn, n) = Some v.
+Proof.
+  intros H a v H1.
+  unfold evalLiteral in *. destruct (nth_error a n) eqn:H2.
+  + specialize (@ntherror_take (bool) a n k b H H2) as H3. now rewrite H3. 
+  + congruence. 
+Qed. 
+
+Lemma bounded_cap_assgn_clause' (c : clause) (n : nat) : varBound_clause n c -> forall (a : assgn) (init v : bool),
+      evalClause' a c (Some init) = Some v -> evalClause' (takeN a n) c (Some init) = Some v. 
+Proof.
+  induction c. 
+  - intros H a init v. cbn; now destruct v. 
+  - intros H assg init v H1. inv H. cbn [evalClause' fold_leftOption] in *.
+    destruct (evalLiteral assg (b, k)) eqn:H5. 
+    + rewrite bounded_cap_assgn_literal with (v := b0). 2-3: assumption.
+      change (evalClause' (takeN assg n) c (Some (init ||b0)) = Some v). now apply IHc.
+    + exfalso. now rewrite fold_leftOption_none_ties_down in H1. 
+Qed. 
+
+Lemma bounded_cap_assgn_clause (c : clause) (n : nat) : varBound_clause n c -> forall (a : assgn) (v : bool),
+      evalClause a c = Some v -> evalClause (takeN a n) c = Some v.
+Proof. intros H a v. now apply bounded_cap_assgn_clause'. Qed. 
+
+Lemma bounded_cap_assgn_cnf' (c : cnf) (n: nat) : varBound_cnf n c -> forall (a : assgn) (init v : bool),
+      evalCnf' a c (Some init) = Some v -> evalCnf' (takeN a n) c (Some init) = Some v.
+Proof.
+  induction c.
+  - intros H a init v. cbn; now destruct v. 
+  - intros H assg init v H1. inv H. cbn [evalCnf' fold_leftOption] in *.
+    destruct (evalClause assg a) eqn:H5.
+    + rewrite bounded_cap_assgn_clause with (v := b). 2-3: assumption.
+      change (evalCnf' (takeN assg n) c (Some (init && b)) = Some v). now apply IHc. 
+    + exfalso. now rewrite fold_leftOption_none_ties_down in H1.
+Qed. 
+
+Lemma bounded_cap_assignment (c:cnf) (n:nat) : varBound_cnf n c -> forall (a :assgn) (v : bool),
+      evalCnf a c = Some v -> evalCnf (takeN a n) c = Some v.
+Proof. intros H a v. now apply bounded_cap_assgn_cnf'. Qed. 
+
+(*now that we've got the tools to verify the verifier, let's build a boolean verifier and prove its correctness*)
+Definition sat_verifierb (input : cnf * assgn) :=
+  let (cn, a) := input in
+    if leb (|a|) (S(cnf_maxVar cn)) then
+      match evalCnf a cn with Some b => b | None => false end
+    else false.
+
+Lemma sat_verifierb_correct (c : cnf) (a : assgn) : reflect (sat_verifier c a) (sat_verifierb (c, a)).
+Proof. 
+  destruct (sat_verifierb (c, a)) eqn:H; constructor. 
+  - unfold sat_verifierb in H. unfold sat_verifier. destruct (leb (|a|) (S (cnf_maxVar c))) eqn:H1.
+    destruct (evalCnf a c) eqn:H2. split; try congruence; dec_bool. all: congruence. 
+  - intros [H1 H2]. cbn in H. apply leb_correct in H2. rewrite H2, H1 in H. congruence. 
+Qed. 
 
 Global Instance term_bool_eqb : computableTime' Bool.eqb (fun _ _ => (1, fun _ _ => (7, tt))). 
 Proof.
@@ -303,8 +409,6 @@ Proof.
   extract. 
   solverec. 
 Qed. 
-
-(*TODO: derive a nice bound under assumptions on the running time of the step function *)
 
 (*we need to factor out the fold step function first and extract it separately *)
 Definition evalClause'_step (a : assgn):=
@@ -368,214 +472,10 @@ Proof.
   extract. solverec. 
 Qed. 
 
-(*fold_left makes verification more ugly, but the runtime functions get easier *)
-Definition clause_maxVar (c : clause) := fold_left (fun acc '(_, v) => Nat.max acc v) c 0. 
-Definition cnf_maxVar (c : cnf) := fold_left (fun acc cl => Nat.max acc (clause_maxVar cl)) c 0.
-
-Lemma varBound_clause_monotonic (c : clause) (n n' : nat) : n <= n' -> varBound_clause n c -> varBound_clause n' c. 
-Proof. intros H1 H2. induction H2. constructor. constructor. lia. auto. Qed. 
-
-Lemma varBound_cnf_monotonic (c : cnf) (n n' : nat) : n <= n' -> varBound_cnf n c -> varBound_cnf n' c.
-Proof.
-  intros H1 H2. induction H2; constructor.
-  now apply varBound_clause_monotonic with (n:= n). assumption. 
-Qed.
-
-Proposition fold_left_maxVar (c : clause) (n :nat) : fold_left (fun acc '(_, v) => Nat.max acc v) c n >= n.
-Proof.
-  revert n; induction c.
-  - intros; cbn; lia. 
-  - intros n. cbn. destruct a. specialize (IHc (Nat.max n n0)). lia.
-Qed. 
-
-Proposition fold_left_maxVar2 (c : clause) (n n' : nat) : n >= n' ->  fold_left (fun acc '(_, v) => Nat.max acc v) c n >= fold_left (fun acc '(_, v) => Nat.max acc v) c n'.
-Proof.
-  revert n n'. induction c.
-  - intros n n'. cbn; lia. 
-  - intros n n' H. cbn; destruct a. apply IHc. lia. 
-Qed. 
-
-Lemma clause_maxVar_bound (c : clause) : varBound_clause (S (clause_maxVar c)) c. 
-Proof.
-  induction c.
-  - cbn. constructor. 
-  - destruct a. constructor. cbn.
-    1: { specialize (fold_left_maxVar c n). lia. } 
-    eapply varBound_clause_monotonic.
-    2: apply IHc. unfold clause_maxVar. cbn. 
-    ring_simplify. assert (n >= 0) by lia. specialize (fold_left_maxVar2 c H). lia. 
-Qed. 
-
-Lemma cnf_maxVar_bound (c : cnf) : varBound_cnf (S (cnf_maxVar c)) c.
-Proof.
-  induction c.
-  - cbn; constructor. 
-  - constructor.
-    1: { cbn. eapply varBound_clause_monotonic. 2: apply clause_maxVar_bound.
-         clear IHc. generalize (clause_maxVar a). induction c.
-         + intros n; cbn; lia. 
-         + intros n; cbn. specialize (IHc (max n (clause_maxVar a0))). lia.  
-       } 
-    eapply varBound_cnf_monotonic. 2: apply IHc. cbn. unfold cnf_maxVar.  
-    pose (step := (fun acc (cl :list (bool * nat)) => Nat.max acc (clause_maxVar cl)) ). 
-    enough (forall n n', n >= n' -> fold_left step c n' <= fold_left step c n).  
-    {assert (0 <= (clause_maxVar a)) by lia. specialize (H (clause_maxVar a) 0 H0). subst step. lia. }
-    clear IHc. induction c. 
-    + intros n n' H. cbn; lia. 
-    + intros n n' H. cbn. apply IHc. unfold step; lia. 
-Qed. 
-
-(*a verifier for SAT. The condition |a| <= S(cnf_maxVar cn) is needed in order to make sure that it rejects certificates that are too long*)
-Definition sat_verifier (cn : cnf) (a : assgn) :=
-  evalCnf a cn = Some true /\ |a| <= S(cnf_maxVar cn).
-
-(*tools needed for the verification of the verifier*)
-Definition takeN (X : Type) := fix rec (l : list X) (n : nat) {struct n} :=
-  match n with 0 => []
-          | S n => match l with [] => []
-                          | (l :: ls) => l :: rec ls n
-                  end
-  end. 
-
-Lemma ntherror_sublist (X : Type) (l l' : list X) (k : nat) (x : X) : (nth_error l k = Some x) -> nth_error (l ++ l') k = Some x. 
-Proof. 
-  revert k. 
-  induction l. 
-  - intros []; cbn; congruence.  
-  - intros k H. destruct k.
-    + cbn in H. destruct l'; now cbn.
-    + cbn. apply IHl. now cbn in H. 
-Qed. 
-
-Lemma takeN_sublist (X : Type) (l : list X) (k k' : nat) (t : list X) : takeN l k = t -> k' >= k -> exists t', takeN l k' = t ++ t'. 
-Proof. 
-  revert k k' t. induction l. 
-  - intros k k' t H1 H2. exists []. destruct k', k; cbn in H1; cbn; rewrite <- H1; firstorder. 
-  - intros k k' t H1 H2. destruct k, k'; cbn in H1; cbn; try rewrite <- H1. firstorder.
-    exists (a :: takeN l k'). firstorder. lia.
-    destruct t; try congruence. 
-    specialize (IHl k k' t). inv H1.  destruct (IHl); try tauto; try lia. exists x0. firstorder. 
-Qed. 
-
-Lemma takeN_more_length (X : Type) (l : list X) (k : nat) : k >= (|l|) ->  takeN l k = l. 
-Proof. 
-  revert k. induction l. 
-  - intros k. cbn. destruct k; tauto. 
-  - intros k. cbn. destruct k; cbn. lia. intros H. rewrite IHl. reflexivity. lia. 
-Qed. 
-
-Lemma takeN_split (X : Type) (l : list X) (k : nat) : exists t, l = takeN l k ++ t.
-Proof.
-  enough (exists t, takeN l (|l|) = takeN l k ++ t). 
-  { destruct H. specialize (@takeN_more_length X l (|l|)) as H2. exists x. now rewrite <- H, H2.   }
-  destruct (lt_eq_lt_dec k (|l|)) as [[H|H] |H].
-  1-2: apply takeN_sublist with (k:=k); try reflexivity; try lia.  
-  exists []. repeat rewrite takeN_more_length. firstorder. all: lia.
-Qed. 
-
-Lemma takeN_length (X : Type) (l :list X) (k : nat) : (|takeN l k|) <= k. 
-Proof. 
-  induction l in k |-*. 
-  - destruct k; cbn; lia. 
-  - destruct k; cbn; try lia. rewrite IHl. lia. 
-Qed. 
-
-Lemma takeN_minlength (X : Type) (l : list X) (n k : nat) : |l| >= k -> n >= k -> |takeN l n| >= k. 
-Proof. 
-  induction l in n, k |-*. 
-  - destruct n; cbn; lia.
-  - cbn. destruct n, k; cbn. 1-3: lia.
-    intros H1 H2. enough (|takeN l n| >= k) by lia. apply IHl; lia.  
-Qed. 
-
-Lemma ntherror_take (X : Type) (l : list X) (k n : nat) (v :X) : k < n -> nth_error l k = Some v -> nth_error (takeN l n) k = Some v. 
-Proof. 
-  specialize (takeN_split l n) as [t H]. intros H1 H2. 
-  (*Proof by contradiction*)
-  destruct (nth_error (takeN l n) k) eqn:H3. 
-  2: { exfalso. 
-       apply nth_error_None in H3. assert (|l| > k) by (now apply nth_error_Some_lt with (x := v)).
-       (*contradiction by H1, H3, H0 *)
-       destruct (takeN_split l k) as [[] H4].
-       - enough (|l| = k) by lia. rewrite H4. enough (|takeN l k| <= k /\ |takeN l k| >= k).
-         {replace (takeN l k ++ []) with (takeN l k) by firstorder. lia. }
-         split. apply takeN_length. apply takeN_minlength. all: lia. 
-       - assert (|takeN l n| = k). enough (|takeN l n| >= k) by lia. apply takeN_minlength; lia. 
-         assert (|takeN l n| >= S k). apply takeN_minlength; lia. lia. 
-  }
-  rewrite H in H2. specialize(Prelim.nthe_app_l t H3) as H4. now rewrite H4 in H2. 
-Qed. 
-
-(*now the wanted results: we can shorten the assignment if this doesn't yield to variables being unbound*)
-Lemma bounded_cap_assgn_literal (n : nat) (sgn : bool) (k : nat) : n < k ->
-  forall (a : assgn) (v : bool), evalLiteral a (sgn, n) = Some v -> evalLiteral (takeN a k) (sgn, n) = Some v.
-Proof.
-  intros H a v H1.
-  unfold evalLiteral in *. destruct (nth_error a n) eqn:H2.
-  + specialize (@ntherror_take (bool) a n k b H H2) as H3. now rewrite H3. 
-  + congruence. 
-Qed. 
-
-Lemma bounded_cap_assgn_clause' (c : clause) (n : nat) : varBound_clause n c -> forall (a : assgn) (init v : bool),
-      evalClause' a c (Some init) = Some v -> evalClause' (takeN a n) c (Some init) = Some v. 
-Proof.
-  induction c. 
-  - intros H a init v. cbn; now destruct v. 
-  - intros H assg init v H1. inv H. cbn [evalClause' fold_leftOption] in *.
-    destruct (evalLiteral assg (b, k)) eqn:H5. 
-    + rewrite bounded_cap_assgn_literal with (v := b0). 2-3: assumption.
-      change (evalClause' (takeN assg n) c (Some (init ||b0)) = Some v). now apply IHc.
-    + exfalso. now rewrite fold_leftOption_none_ties_down in H1. 
-Qed. 
-
-Lemma bounded_cap_assgn_clause (c : clause) (n : nat) : varBound_clause n c -> forall (a : assgn) (v : bool),
-      evalClause a c = Some v -> evalClause (takeN a n) c = Some v.
-Proof. intros H a v. now apply bounded_cap_assgn_clause'. Qed. 
-
-Lemma bounded_cap_assgn_cnf' (c : cnf) (n: nat) : varBound_cnf n c -> forall (a : assgn) (init v : bool),
-      evalCnf' a c (Some init) = Some v -> evalCnf' (takeN a n) c (Some init) = Some v.
-Proof.
-  induction c.
-  - intros H a init v. cbn; now destruct v. 
-  - intros H assg init v H1. inv H. cbn [evalCnf' fold_leftOption] in *.
-    destruct (evalClause assg a) eqn:H5.
-    + rewrite bounded_cap_assgn_clause with (v := b). 2-3: assumption.
-      change (evalCnf' (takeN assg n) c (Some (init && b)) = Some v). now apply IHc. 
-    + exfalso. now rewrite fold_leftOption_none_ties_down in H1.
-Qed. 
-
-Lemma bounded_cap_assignment (c:cnf) (n:nat) : varBound_cnf n c -> forall (a :assgn) (v : bool),
-      evalCnf a c = Some v -> evalCnf (takeN a n) c = Some v.
-Proof. intros H a v. now apply bounded_cap_assgn_cnf'. Qed. 
-
-(*now that we've got the tools to verify the verifier, let's build a boolean verifier and prove its correctness*)
-Definition sat_verifierb (input : cnf * assgn) :=
-  let (cn, a) := input in
-    if leb (|a|) (S(cnf_maxVar cn)) then
-      match evalCnf a cn with Some b => b | None => false end
-    else false.
-
-Lemma sat_verifierb_correct (c : cnf) (a : assgn) : reflect (sat_verifier c a) (sat_verifierb (c, a)).
-Proof. 
-  destruct (sat_verifierb (c, a)) eqn:H; constructor. 
-  - unfold sat_verifierb in H. unfold sat_verifier. destruct (leb (|a|) (S (cnf_maxVar c))) eqn:H1.
-    destruct (evalCnf a c) eqn:H2. split; try congruence; dec_bool. all: congruence. 
-  - intros [H1 H2]. cbn in H. apply leb_correct in H2. rewrite H2, H1 in H. congruence. 
-Qed. 
-
 (*extraction of the verifier *)
-Fixpoint fold_left_time X Y (f : X -> Y -> X) (t__f : X -> unit -> nat * (Y -> unit -> nat * unit)) (l : list Y) (acc : X) :=
-  (match l with
-       | [] => 4
-       | (l :: ls) => callTime2 t__f acc l + 15 + fold_left_time f t__f ls (f acc l)
-       end ).
 
-Instance term_fold_left (X: Type) (Y : Type) `{registered X} `{registered Y} :
-  computableTime' (@fold_left X Y) (fun f fT => (5, fun l _ => (5, fun acc _ => (fold_left_time f fT l acc, tt)))). 
-Proof.
-  extract. 
-  solverec. 
-Qed. 
+
+
 
 Definition clause_maxVar_step := fun (acc : nat) (l : literal) => let '(_, v) := l in max acc v. 
 Instance term_clause_maxVar_step : computableTime' clause_maxVar_step (fun acc _ => (1, fun l _ => (let '(_, v):= l in 18 + 15 * min acc v, tt))). 
